Integrating specification language support into ./language/move-prover.
This adapts concepts of David's spec language prototype and combines it with Sam's new spec parsing support in the Move parser. It also refactors and cleans up some of the tool level plumbing for the move prover, so we can more productively iterate on it.

The spec language support is not complete, as indicated the by TODO markers in the source.

Quite a bit work in this PR is about getting a better command line interface and test support for MVP (the Move Prover). I apologize to have not split this out. If you are mostly interested in the actual spec translation (and its open problems), see `src/spec_translator.rs`, and the related test output at `tests\goldenfiles\test-specs.bpl`.

language/move-prover/bytecode-to-boogie/src/driver.rs
@@ -1,0 +1,189 @@
+// Copyright (c) The Libra Core Contributors
+// SPDX-License-Identifier: Apache-2.0
+
+#![forbid(unsafe_code)]
+
+use crate::cli::{abort_on_error, Options, INLINE_PRELUDE};
+use crate::translator::{BoogieTranslator, FunctionInfo, ModuleInfo};
+use bytecode_source_map::source_map::SourceMap;
+use bytecode_verifier::VerifiedModule;
+use ir_to_bytecode::compiler::compile_module;
+use ir_to_bytecode::parser::ast::{Loc, ModuleDefinition};
+use ir_to_bytecode::parser::parse_module;
+use itertools::Itertools;
+use libra_types::account_address::AccountAddress;
+use log::{debug, error, info};
+use std::fs;
+use std::process::Command;
+
+/// Content of the default prelude.
+const DEFAULT_PRELUDE: &[u8] = include_bytes!("bytecode_instrs.bpl");
+
+/// Represents the driver for translation.
+pub struct Driver<'app> {
+    /// Options passed via the cli.
+    options: &'app Options,
+    /// List of module specs.
+    module_infos: Vec<ModuleInfo>,
+    /// List of verified modules.
+    verified_modules: Vec<VerifiedModule>,
+    /// Source position map.
+    source_map: SourceMap<Loc>,
+    /// Generated output.
+    pub output: String,
+}
+
+impl<'app> Driver<'app> {
+    pub fn new(options: &'app Options) -> Self {
+        Driver {
+            options,
+            module_infos: vec![],
+            verified_modules: vec![],
+            source_map: vec![],
+            output: String::new(),
+        }
+    }
+
+    /// Runs standard translation. When this finishes, the generated code is in `self.output`.
+    pub fn run(&mut self) {
+        self.load_modules(&self.options.mvir_sources);
+        self.add_prelude();
+        self.translate_modules();
+        // write resulting code
+        info!("writing boogie to {}", self.options.output_path);
+        abort_on_error(
+            fs::write(&self.options.output_path, &self.output),
+            "cannot write boogie file",
+        );
+        if !self.options.generate_only {
+            self.call_boogie(&self.options.output_path);
+        }
+    }
+
+    /// Runs translation in a test context. Instead of writing output to a file, returns
+    /// a pair of the prelude and the actual translated code.
+    pub fn run_for_test(&mut self) -> (String, String) {
+        self.load_modules(&self.options.mvir_sources);
+        self.add_prelude();
+        // Extract the prelude from the generated output, as we want to return it in a separate
+        // string.
+        let prelude = std::mem::replace(&mut self.output, String::new());
+        self.translate_modules();
+        (prelude, std::mem::replace(&mut self.output, String::new()))
+    }
+
+    /// Compiles the list of mvir modules and adds them to the state. On errors, this
+    /// reports and aborts. Nothing will be added to the output yet.
+    pub fn load_modules(&mut self, file_names: &[String]) {
+        // TODO: make the address configurable.
+        let address = AccountAddress::default();
+        for (index, file_name) in file_names.iter().enumerate() {
+            info!("analyzing {}", file_name);
+            // Parse module.
+            let code = abort_on_error(fs::read_to_string(file_name), "cannot read mvir file");
+            let parsed_module = abort_on_error(parse_module(&code), "mvir parsing errors");
+            let name = parsed_module.name.as_inner().to_string();
+
+            // Extract specifications from module.
+            let specs = self.extract_function_infos(&parsed_module);
+
+            // Compile module.
+            let (compiled_module, source_map) = abort_on_error(
+                compile_module(address, parsed_module, &self.verified_modules),
+                "mvir compilation errors",
+            );
+
+            // Verify module byte code.
+            let verified_module = abort_on_error(
+                VerifiedModule::new(compiled_module)
+                    // As an error message, produce a line separated list of VMStatus.
+                    .map_err(|(_, sv)| sv.iter().map(|s| format!("{:?}", s)).join("\n")),
+                "mvir verification errors",
+            );
+
+            // Store result.
+            self.verified_modules.push(verified_module);
+            self.module_infos.push(ModuleInfo {
+                index,
+                name,
+                function_infos: specs,
+            });
+            self.source_map.push(source_map);
+        }
+    }
+
+    /// Extract function infos from the given parsed module.
+    fn extract_function_infos(&self, parsed_module: &ModuleDefinition) -> Vec<FunctionInfo> {
+        let mut result = vec![];
+        for (index, (name, def)) in parsed_module.functions.iter().enumerate() {
+            let function_name = name.as_inner().as_str().to_string();
+            let type_arg_names = def
+                .value
+                .signature
+                .type_formals
+                .iter()
+                .map(|(v, _)| v.value.name().as_str().to_string())
+                .collect();
+            let arg_names = def
+                .value
+                .signature
+                .formals
+                .iter()
+                .map(|(v, _)| v.value.name().as_str().to_string())
+                .collect();
+            result.push(FunctionInfo {
+                index,
+                name: function_name,
+                type_arg_names,
+                arg_names,
+                specification: def.value.specifications.clone(),
+            });
+        }
+        result
+    }
+
+    /// Adds the prelude to the generated output.
+    pub fn add_prelude(&mut self) {
+        self.output.push_str(&format!(
+            "\n// ** prelude from {}\n\n",
+            self.options.prelude_path
+        ));
+        if self.options.prelude_path == INLINE_PRELUDE {
+            info!("using inline prelude");
+            self.output
+                .push_str(&String::from_utf8_lossy(DEFAULT_PRELUDE));
+        } else {
+            info!("using prelude at {}", &self.options.prelude_path);
+            let content = abort_on_error(
+                fs::read_to_string(&self.options.prelude_path),
+                "cannot read prelude file",
+            );
+            self.output.push_str(&content);
+        }
+    }
+
+    /// Translates all modules.
+    pub fn translate_modules(&mut self) {
+        self.output.push_str(
+            &BoogieTranslator::new(&self.verified_modules, &self.module_infos, &self.source_map)
+                .translate(),
+        );
+    }
+
+    /// Calls boogie on the given file.
+    pub fn call_boogie(&self, boogie_file: &str) -> bool {
+        let args = self.options.get_boogie_command(boogie_file);
+        info!("calling boogie");
+        debug!("command line: {}", args.iter().join(" "));
+        let status = abort_on_error(
+            Command::new(&args[0]).args(&args[1..]).status(),
+            "error executing boogie",
+        );
+        if !status.success() {
+            error!("boogie exited with status {}", status.code().unwrap());
+            false
+        } else {
+            true
+        }
+    }
+}
